Fix a bunch of translation and struct bugs
This commit combines many fixes from trying to get logging2 to
typecheck. That process is almost complete, except that we need some
typing rules for maps.

Some of the bugs fixed include:
- SliceAppend appended slices rather than a single element
- struct accessors were generated incorrectly
- there was no way to typecheck the slice operations
- typechecking unfolded slice.T, which sometimes prevented it from
  working

src/go_lang/prelude.v
@@ -8,10 +8,11 @@ From Perennial.go_lang Require Export
 
 Inductive LockMode := Reader | Writer.
 Definition uint64_to_string {ext: ext_op}: val := λ: <>, #().
+Definition lockRefT := refT intT.
 
 Module Data.
   Section go_lang.
-    Context {ext:ext_op}.
+    Context `{ext_ty:ext_types}.
     Definition stringToBytes: val := λ: <>, #().
     Definition bytesToString: val := λ: <>, #().
     Definition sliceAppendSlice: val := λ: <>, #().
@@ -19,11 +20,29 @@ Module Data.
     Definition mapIter: val := λ: <>, #().
     Definition mapClear: val := λ: <>, #().
     Definition randomUint64: val := λ: <>, #().
-    Definition newLock: val := λ: <>, #().
+
+    Definition newLock: val := λ: <>, ref #0.
+    Theorem newLock_t: ⊢ newLock : (unitT -> lockRefT).
+    Proof.
+      typecheck.
+    Qed.
+
     Definition lockRelease (m: LockMode): val := λ: <>, #().
+    Theorem lockRelease_t m: ⊢ lockRelease m : (lockRefT -> unitT).
+    Proof.
+      typecheck.
+    Qed.
+
     Definition lockAcquire (m: LockMode): val := λ: <>, #().
+    Theorem lockAcquire_t m: ⊢ lockAcquire m : (lockRefT -> unitT).
+    Proof.
+      typecheck.
+    Qed.
   End go_lang.
 End Data.
+
+Opaque Data.newLock Data.lockRelease Data.lockAcquire.
+Hint Resolve Data.newLock_t Data.lockRelease_t Data.lockAcquire_t : types.
 
 Module FS.
   Section go_lang.
@@ -51,5 +70,3 @@ Module Globals.
     Definition setX: val := λ: <>, #().
   End go_lang.
 End Globals.
-
-Definition lockRefT := refT intT.
