src/go_lang/examples/logging2.v
@@ -34,9 +34,6 @@ Definition Log__writeHdr: val :=
     let: "hdr" := NewSlice byteT #4096 in
     UInt64Put "hdr" "len";;
     disk.Write LOGCOMMIT "hdr".
-Theorem Log__writeHdr_t: ⊢ Log__writeHdr : (Log.T -> intT -> unitT).
-Proof. typecheck. Qed.
-Hint Resolve Log__writeHdr_t : types.
 
 Definition Init: val :=
   λ: "logSz",
@@ -51,31 +48,22 @@ Definition Init: val :=
     ] in
     Log__writeHdr "log" #0;;
     "log".
-Theorem Init_t: ⊢ Init : (intT -> Log.T).
-Proof. typecheck. Qed.
-Hint Resolve Init_t : types.
 
 Definition Log__readHdr: val :=
   λ: "log",
     let: "hdr" := disk.Read LOGCOMMIT in
     let: "disklen" := UInt64Get "hdr" in
     "disklen".
-Theorem Log__readHdr_t: ⊢ Log__readHdr : (Log.T -> intT).
-Proof. typecheck. Qed.
-Hint Resolve Log__readHdr_t : types.
 
 Definition Log__readBlocks: val :=
   λ: "log" "len",
     let: "blks" := ref (NewSlice disk.blockT #0) in
     let: "i" := ref #0 in
-    for: (!"i" < "len"); ("i" <- !"i" + #1) :=
+    (for: (!"i" < "len"); ("i" <- !"i" + #1) :=
       let: "blk" := disk.Read (LOGSTART + !"i") in
       "blks" <- SliceAppend !"blks" "blk";;
-      Continue;;
+      Continue);;
     !"blks".
-Theorem Log__readBlocks_t: ⊢ Log__readBlocks : (Log.T -> intT -> slice.T disk.blockT).
-Proof. typecheck. Qed.
-Hint Resolve Log__readBlocks_t : types.
 
 Definition Log__Read: val :=
   λ: "log",
@@ -84,25 +72,19 @@ Definition Log__Read: val :=
     let: "blks" := Log__readBlocks "log" "disklen" in
     Data.lockRelease Writer (Log.get "logLock" "log");;
     "blks".
-Theorem Log__Read_t: ⊢ Log__Read : (Log.T -> slice.T disk.blockT).
-Proof. typecheck. Qed.
-Hint Resolve Log__Read_t : types.
 
 Definition Log__memWrite: val :=
   λ: "log" "l",
     let: "n" := slice.len "l" in
     let: "i" := ref #0 in
-    for: (!"i" < "n"); ("i" <- !"i" + #1) :=
+    (for: (!"i" < "n"); ("i" <- !"i" + #1) :=
       Log.get "memLog" "log" <- SliceAppend (!(Log.get "memLog" "log")) (SliceGet "l" !"i");;
-      Continue.
-Theorem Log__memWrite_t: ⊢ Log__memWrite : (Log.T -> slice.T disk.blockT -> unitT).
-Proof. typecheck. Qed.
-Hint Resolve Log__memWrite_t : types.
+      Continue).
 
 Definition Log__memAppend: val :=
   λ: "log" "l",
     Data.lockAcquire Writer (Log.get "memLock" "log");;
-    if: !(Log.get "memLen" "log") + slice.len "l" ≥ Log.get "logSz" "log"
+    (if: !(Log.get "memLen" "log") + slice.len "l" ≥ Log.get "logSz" "log"
     then
       Data.lockRelease Writer (Log.get "memLock" "log");;
       (#false, #0)
@@ -112,10 +94,7 @@ Definition Log__memAppend: val :=
       Log.get "memLen" "log" <- "n";;
       Log.get "memTxnNxt" "log" <- !(Log.get "memTxnNxt" "log") + #1;;
       Data.lockRelease Writer (Log.get "memLock" "log");;
-      (#true, "txn").
-Theorem Log__memAppend_t: ⊢ Log__memAppend : (Log.T -> slice.T disk.blockT -> (boolT * intT)).
-Proof. typecheck. Qed.
-Hint Resolve Log__memAppend_t : types.
+      (#true, "txn")).
 
 (* XXX just an atomic read? *)
 Definition Log__readLogTxnNxt: val :=
@@ -124,46 +103,34 @@ Definition Log__readLogTxnNxt: val :=
     let: "n" := !(Log.get "logTxnNxt" "log") in
     Data.lockRelease Writer (Log.get "memLock" "log");;
     "n".
-Theorem Log__readLogTxnNxt_t: ⊢ Log__readLogTxnNxt : (Log.T -> intT).
-Proof. typecheck. Qed.
-Hint Resolve Log__readLogTxnNxt_t : types.
 
 Definition Log__diskAppendWait: val :=
   λ: "log" "txn",
     Skip;;
-    for: (#true); (Skip) :=
+    (for: (#true); (Skip) :=
       let: "logtxn" := Log__readLogTxnNxt "log" in
-      if: "txn" < "logtxn"
+      (if: "txn" < "logtxn"
       then Break
-      else Continue.
-Theorem Log__diskAppendWait_t: ⊢ Log__diskAppendWait : (Log.T -> intT -> unitT).
-Proof. typecheck. Qed.
-Hint Resolve Log__diskAppendWait_t : types.
+      else Continue)).
 
 Definition Log__Append: val :=
   λ: "log" "l",
     let: ("ok", "txn") := Log__memAppend "log" "l" in
-    if: "ok"
+    (if: "ok"
     then
       Log__diskAppendWait "log" "txn";;
       #()
-    else #();;
+    else #());;
     "ok".
-Theorem Log__Append_t: ⊢ Log__Append : (Log.T -> slice.T disk.blockT -> boolT).
-Proof. typecheck. Qed.
-Hint Resolve Log__Append_t : types.
 
 Definition Log__writeBlocks: val :=
   λ: "log" "l" "pos",
     let: "n" := slice.len "l" in
     let: "i" := ref #0 in
-    for: (!"i" < "n"); ("i" <- !"i" + #1) :=
+    (for: (!"i" < "n"); ("i" <- !"i" + #1) :=
       let: "bk" := SliceGet "l" !"i" in
       disk.Write ("pos" + !"i") "bk";;
-      Continue.
-Theorem Log__writeBlocks_t: ⊢ Log__writeBlocks : (Log.T -> slice.T disk.blockT -> intT -> unitT).
-Proof. typecheck. Qed.
-Hint Resolve Log__writeBlocks_t : types.
+      Continue).
 
 Definition Log__diskAppend: val :=
   λ: "log",
@@ -179,19 +146,13 @@ Definition Log__diskAppend: val :=
     Log__writeHdr "log" "memlen";;
     Log.get "logTxnNxt" "log" <- "memnxt";;
     Data.lockRelease Writer (Log.get "logLock" "log").
-Theorem Log__diskAppend_t: ⊢ Log__diskAppend : (Log.T -> unitT).
-Proof. typecheck. Qed.
-Hint Resolve Log__diskAppend_t : types.
 
 Definition Log__Logger: val :=
   λ: "log",
     Skip;;
-    for: (#true); (Skip) :=
+    (for: (#true); (Skip) :=
       Log__diskAppend "log";;
-      Continue.
-Theorem Log__Logger_t: ⊢ Log__Logger : (Log.T -> unitT).
-Proof. typecheck. Qed.
-Hint Resolve Log__Logger_t : types.
+      Continue).
 
 Module Txn.
   Definition S := struct.new [
@@ -213,39 +174,31 @@ Definition Begin: val :=
       "blks" ::= ref (zero_val (mapT disk.blockT))
     ] in
     "txn".
-Theorem Begin_t: ⊢ Begin : (refT Log.T -> Txn.T).
-Proof. typecheck. Qed.
-Hint Resolve Begin_t : types.
 
 Definition Txn__Write: val :=
   λ: "txn" "addr" "blk",
+    let: "ret" := ref #true in
     let: (<>, "ok") := MapGet (!(Txn.get "blks" "txn")) "addr" in
-    if: "ok"
+    (if: "ok"
     then
       MapInsert (!(Txn.get "blks" "txn")) "addr" !"blk";;
       #()
-    else #();;
-    if: ~ "ok"
+    else #());;
+    (if: ~ "ok"
     then
-      if: "addr" = LOGMAXBLK
-      then #false
-      else MapInsert (!(Txn.get "blks" "txn")) "addr" !"blk";;
+      (if: "addr" = LOGMAXBLK
+      then "ret" <- #false
+      else MapInsert (!(Txn.get "blks" "txn")) "addr" !"blk");;
       #()
-    else #();;
-    #true.
-Theorem Txn__Write_t: ⊢ Txn__Write : (Txn.T -> intT -> refT disk.blockT -> boolT).
-Proof. typecheck. Qed.
-Hint Resolve Txn__Write_t : types.
+    else #());;
+    !"ret".
 
 Definition Txn__Read: val :=
   λ: "txn" "addr",
     let: ("v", "ok") := MapGet (!(Txn.get "blks" "txn")) "addr" in
-    if: "ok"
+    (if: "ok"
     then "v"
-    else disk.Read ("addr" + LOGEND).
-Theorem Txn__Read_t: ⊢ Txn__Read : (Txn.T -> intT -> disk.blockT).
-Proof. typecheck. Qed.
-Hint Resolve Txn__Read_t : types.
+    else disk.Read ("addr" + LOGEND)).
 
 Definition Txn__Commit: val :=
   λ: "txn",
@@ -254,6 +207,3 @@ Definition Txn__Commit: val :=
       "blks" <- SliceAppend !"blks" "v");;
     let: "ok" := Log__Append (!(Txn.get "log" "txn")) !"blks" in
     "ok".
-Theorem Txn__Commit_t: ⊢ Txn__Commit : (Txn.T -> boolT).
-Proof. typecheck. Qed.
-Hint Resolve Txn__Commit_t : types.
